got rid of split-at-mut

libcrux-ml-kem/proofs/fstar/extraction/Libcrux_ml_kem.Constants.fsti
@@ -17,6 +17,9 @@ let v_COEFFICIENTS_IN_RING_ELEMENT: usize = Rust_primitives.Hax.dropped_body
 
 let v_CPA_PKE_KEY_GENERATION_SEED_SIZE: usize = Rust_primitives.Hax.dropped_body
 
+/// Field modulus: 3329
+let v_FIELD_MODULUS: i16 = Rust_primitives.Hax.dropped_body
+
 /// SHA3 512 digest size
 let v_G_DIGEST_SIZE: usize = Rust_primitives.Hax.dropped_body
 
@@ -25,6 +28,3 @@ let v_H_DIGEST_SIZE: usize = Rust_primitives.Hax.dropped_body
 
 /// The size of an ML-KEM shared secret.
 let v_SHARED_SECRET_SIZE: usize = Rust_primitives.Hax.dropped_body
-
-/// Field modulus: 3329
-let v__FIELD_MODULUS: i16 = Rust_primitives.Hax.dropped_body
