libcrux-ml-kem/proofs/fstar/extraction/Libcrux_ml_kem.Hash_functions.Neon.fsti
@@ -49,7 +49,7 @@ let impl (v_K: usize) : Libcrux_ml_kem.Hash_functions.t_Hash t_Simd128Hash v_K =
     (fun
         (v_LEN: usize)
         (input: t_Array (t_Array u8 (sz 33)) v_K)
-        (out1: t_Array (t_Array u8 v_LEN) v_K)
+        (out4: t_Array (t_Array u8 v_LEN) v_K)
         ->
         true);
     f_PRFxN
@@ -71,41 +71,127 @@ let impl (v_K: usize) : Libcrux_ml_kem.Hash_functions.t_Hash t_Simd128Hash v_K =
         let out:t_Array (t_Array u8 v_LEN) v_K =
           Rust_primitives.Hax.repeat (Rust_primitives.Hax.repeat 0uy v_LEN <: t_Array u8 v_LEN) v_K
         in
-        let _:Prims.unit =
+        let out0:t_Array u8 v_LEN = Rust_primitives.Hax.repeat 0uy v_LEN in
+        let out1:t_Array u8 v_LEN = Rust_primitives.Hax.repeat 0uy v_LEN in
+        let out2:t_Array u8 v_LEN = Rust_primitives.Hax.repeat 0uy v_LEN in
+        let out3:t_Array u8 v_LEN = Rust_primitives.Hax.repeat 0uy v_LEN in
+        let out, out0, out1, out2, out3:(t_Array (t_Array u8 v_LEN) v_K & t_Array u8 v_LEN &
+          t_Array u8 v_LEN &
+          t_Array u8 v_LEN &
+          t_Array u8 v_LEN) =
           match cast (v_K <: usize) <: u8 with
           | 2uy ->
-            Rust_primitives.Hax.failure ""
-              "{\n        let Tuple2(out0, out1): tuple2<&mut [[int; LEN]], &mut [[int; LEN]]> = {\n            core::slice::impl__split_at_mut::<[int; LEN]>(rust_primitives::unsize(&mut (out)), 1)\n        };\n        {\n            let _: tuple0 = {\n                libcrux_sha3::neon::x2::shake256(\n                    rust_primitives::unsize(\n                        &(deref(&(core::ops::index::Index::index(deref(input), 0)))),\n                    ),\n                    rust_primitives::unsize(\n                        &(deref(&(core::ops::index::Index::index(deref(input), 1)))),\n                    ),\n                    rust_primitives::unsize(\n                        &mut (deref(&mut (core::ops::index::Index::index(deref(out0), 0)))),\n                    ),\n                    rust_primitives::unsize(\n                        &mut (deref(&mut (core::ops::index::Index::index(deref(out1), 0)))),\n                    ),\n                )\n            };\n            Tuple0\n        }\n    }"
-
+            let tmp0, tmp1:(t_Array u8 v_LEN & t_Array u8 v_LEN) =
+              Libcrux_sha3.Neon.X2.shake256 (Rust_primitives.unsize (input.[ sz 0 ]
+                      <:
+                      t_Array u8 (sz 33))
+                  <:
+                  t_Slice u8)
+                (Rust_primitives.unsize (input.[ sz 1 ] <: t_Array u8 (sz 33)) <: t_Slice u8)
+                out0
+                out1
+            in
+            let out0:t_Array u8 v_LEN = tmp0 in
+            let out1:t_Array u8 v_LEN = tmp1 in
+            let _:Prims.unit = () in
+            let out:t_Array (t_Array u8 v_LEN) v_K =
+              Rust_primitives.Hax.Monomorphized_update_at.update_at_usize out (sz 0) out0
+            in
+            let out:t_Array (t_Array u8 v_LEN) v_K =
+              Rust_primitives.Hax.Monomorphized_update_at.update_at_usize out (sz 1) out1
+            in
+            out, out0, out1, out2, out3
+            <:
+            (t_Array (t_Array u8 v_LEN) v_K & t_Array u8 v_LEN & t_Array u8 v_LEN & t_Array u8 v_LEN &
+              t_Array u8 v_LEN)
           | 3uy ->
-            let extra:t_Array u8 v_LEN = Rust_primitives.Hax.repeat 0uy v_LEN in
-            Rust_primitives.Hax.failure ""
-              "{\n        let Tuple2(out0, out12): tuple2<&mut [[int; LEN]], &mut [[int; LEN]]> = {\n            core::slice::impl__split_at_mut::<[int; LEN]>(rust_primitives::unsize(&mut (out)), 1)\n        };\n        {\n            let Tuple2(out1, out2): tuple2<&mut [[int; LEN]], &mut [[int; LEN]]> =\n                { core::slice::impl__split_at_mut::<[int; LEN]>(&mut (deref(out12)), 1) };\n            {\n                let _: tuple0 = {\n                    libcrux_sha3::neon::x2::shake256(\n                        rust_primitives::unsize(\n                            &(deref(&(core::ops::index::Index::index(deref(input), 0)))),\n                        ),\n                        rust_primitives::unsize(\n                            &(deref(&(core::ops::index::Index::index(deref(input), 1)))),\n                        ),\n                        rust_primitives::unsize(\n                            &mut (deref(&mut (core::ops::index::Index::index(deref(out0), 0)))),\n                        ),\n                        rust_primitives::unsize(\n                            &mut (deref(&mut (core::ops::index::Index::index(deref(out1), 0)))),\n                        ),\n                    )\n                };\n                {\n                    let _: tuple0 = {\n                        libcrux_sha3::neon::x2::shake256(\n                            rust_primitives::unsize(\n                                &(deref(&(core::ops::index::Index::index(deref(input), 2)))),\n                            ),\n                            rust_primitives::unsize(\n                                &(deref(&(core::ops::index::Index::index(deref(input), 2)))),\n                            ),\n                            rust_primitives::unsize(\n                                &mut (deref(&mut (core::ops::index::Index::index(deref(out2), 0)))),\n                            ),\n                            rust_primitives::unsize(&mut (deref(&mut (extra)))),\n                        )\n                    };\n                    Tuple0\n                }\n            }\n        }\n    }"
-
+            let tmp0, tmp1:(t_Array u8 v_LEN & t_Array u8 v_LEN) =
+              Libcrux_sha3.Neon.X2.shake256 (Rust_primitives.unsize (input.[ sz 0 ]
+                      <:
+                      t_Array u8 (sz 33))
+                  <:
+                  t_Slice u8)
+                (Rust_primitives.unsize (input.[ sz 1 ] <: t_Array u8 (sz 33)) <: t_Slice u8)
+                out0
+                out1
+            in
+            let out0:t_Array u8 v_LEN = tmp0 in
+            let out1:t_Array u8 v_LEN = tmp1 in
+            let _:Prims.unit = () in
+            let tmp0, tmp1:(t_Array u8 v_LEN & t_Array u8 v_LEN) =
+              Libcrux_sha3.Neon.X2.shake256 (Rust_primitives.unsize (input.[ sz 2 ]
+                      <:
+                      t_Array u8 (sz 33))
+                  <:
+                  t_Slice u8)
+                (Rust_primitives.unsize (input.[ sz 2 ] <: t_Array u8 (sz 33)) <: t_Slice u8)
+                out2
+                out3
+            in
+            let out2:t_Array u8 v_LEN = tmp0 in
+            let out3:t_Array u8 v_LEN = tmp1 in
+            let _:Prims.unit = () in
+            let out:t_Array (t_Array u8 v_LEN) v_K =
+              Rust_primitives.Hax.Monomorphized_update_at.update_at_usize out (sz 0) out0
+            in
+            let out:t_Array (t_Array u8 v_LEN) v_K =
+              Rust_primitives.Hax.Monomorphized_update_at.update_at_usize out (sz 1) out1
+            in
+            let out:t_Array (t_Array u8 v_LEN) v_K =
+              Rust_primitives.Hax.Monomorphized_update_at.update_at_usize out (sz 2) out2
+            in
+            out, out0, out1, out2, out3
+            <:
+            (t_Array (t_Array u8 v_LEN) v_K & t_Array u8 v_LEN & t_Array u8 v_LEN & t_Array u8 v_LEN &
+              t_Array u8 v_LEN)
           | 4uy ->
-            Rust_primitives.Hax.failure ""
-              "{\n        let Tuple2(out0, out123): tuple2<&mut [[int; LEN]], &mut [[int; LEN]]> = {\n            core::slice::impl__split_at_mut::<[int; LEN]>(rust_primitives::unsize(&mut (out)), 1)\n        };\n        {\n            let Tuple2(out1, out23): tuple2<&mut [[int; LEN]], &mut [[int; LEN]]> =\n                { core::slice::impl__split_at_mut::<[int; LEN]>(&mut (deref(out123)), 1) };\n            {\n                let Tuple2(out2, out3): tuple2<&mut [[int; LEN]], &mut [[int; LEN]]> =\n                    { core::slice::impl__split_at_mut::<[int; LEN]>(&mut (deref(out23)), 1) };\n                {\n                    let _: tuple0 = {\n                        libcrux_sha3::neon::x2::shake256(\n                            rust_primitives::unsize(\n                                &(deref(&(core::ops::index::Index::index(deref(input), 0)))),\n                            ),\n                            rust_primitives::unsize(\n                                &(deref(&(core::ops::index::Index::index(deref(input), 1)))),\n                            ),\n                            rust_primitives::unsize(\n                                &mut (deref(&mut (core::ops::index::Index::index(deref(out0), 0)))),\n                            ),\n                            rust_primitives::unsize(\n                                &mut (deref(&mut (core::ops::index::Index::index(deref(out1), 0)))),\n                            ),\n                        )\n                    };\n                    {\n                        let _: tuple0 = {\n                            libcrux_sha3::neon::x2::shake256(\n                                rust_primitives::unsize(\n                                    &(deref(&(core::ops::index::Index::index(deref(input), 2)))),\n                                ),\n                                rust_primitives::unsize(\n                                    &(deref(&(core::ops::index::Index::index(deref(input), 3)))),\n                                ),\n                                rust_primitives::unsize(\n                                    &mut (deref(\n                                        &mut (core::ops::index::Index::index(deref(out2), 0)),\n                                    )),\n                                ),\n                                rust_primitives::unsize(\n                                    &mut (deref(\n                                        &mut (core::ops::index::Index::index(deref(out3), 0)),\n                                    )),\n                                ),\n                            )\n                        };\n                        Tuple0\n                    }\n                }\n            }\n        }\n    }"
-
+            let tmp0, tmp1:(t_Array u8 v_LEN & t_Array u8 v_LEN) =
+              Libcrux_sha3.Neon.X2.shake256 (Rust_primitives.unsize (input.[ sz 0 ]
+                      <:
+                      t_Array u8 (sz 33))
+                  <:
+                  t_Slice u8)
+                (Rust_primitives.unsize (input.[ sz 1 ] <: t_Array u8 (sz 33)) <: t_Slice u8)
+                out0
+                out1
+            in
+            let out0:t_Array u8 v_LEN = tmp0 in
+            let out1:t_Array u8 v_LEN = tmp1 in
+            let _:Prims.unit = () in
+            let tmp0, tmp1:(t_Array u8 v_LEN & t_Array u8 v_LEN) =
+              Libcrux_sha3.Neon.X2.shake256 (Rust_primitives.unsize (input.[ sz 2 ]
+                      <:
+                      t_Array u8 (sz 33))
+                  <:
+                  t_Slice u8)
+                (Rust_primitives.unsize (input.[ sz 3 ] <: t_Array u8 (sz 33)) <: t_Slice u8)
+                out2
+                out3
+            in
+            let out2:t_Array u8 v_LEN = tmp0 in
+            let out3:t_Array u8 v_LEN = tmp1 in
+            let _:Prims.unit = () in
+            let out:t_Array (t_Array u8 v_LEN) v_K =
+              Rust_primitives.Hax.Monomorphized_update_at.update_at_usize out (sz 0) out0
+            in
+            let out:t_Array (t_Array u8 v_LEN) v_K =
+              Rust_primitives.Hax.Monomorphized_update_at.update_at_usize out (sz 1) out1
+            in
+            let out:t_Array (t_Array u8 v_LEN) v_K =
+              Rust_primitives.Hax.Monomorphized_update_at.update_at_usize out (sz 2) out2
+            in
+            let out:t_Array (t_Array u8 v_LEN) v_K =
+              Rust_primitives.Hax.Monomorphized_update_at.update_at_usize out (sz 3) out3
+            in
+            out, out0, out1, out2, out3
+            <:
+            (t_Array (t_Array u8 v_LEN) v_K & t_Array u8 v_LEN & t_Array u8 v_LEN & t_Array u8 v_LEN &
+              t_Array u8 v_LEN)
           | _ ->
-            Rust_primitives.Hax.never_to_any (Core.Panicking.panic_fmt (Core.Fmt.impl_2__new_v1 (Rust_primitives.unsize
-                          (let list =
-                              [
-                                "internal error: entered unreachable code: Only 2, 3, or 4 are supported for N"
-                              ]
-                            in
-                            FStar.Pervasives.assert_norm (Prims.eq2 (List.Tot.length list) 1);
-                            Rust_primitives.Hax.array_of_list 1 list)
-                        <:
-                        t_Slice string)
-                      (Rust_primitives.unsize (Core.Fmt.Rt.impl_1__none ()
-                            <:
-                            t_Array Core.Fmt.Rt.t_Argument (sz 0))
-                        <:
-                        t_Slice Core.Fmt.Rt.t_Argument)
-                    <:
-                    Core.Fmt.t_Arguments)
-                <:
-                Rust_primitives.Hax.t_Never)
+            out, out0, out1, out2, out3
+            <:
+            (t_Array (t_Array u8 v_LEN) v_K & t_Array u8 v_LEN & t_Array u8 v_LEN & t_Array u8 v_LEN &
+              t_Array u8 v_LEN)
         in
         out);
     f_shake128_init_absorb_pre = (fun (input: t_Array (t_Array u8 (sz 34)) v_K) -> true);
@@ -207,7 +293,7 @@ let impl (v_K: usize) : Libcrux_ml_kem.Hash_functions.t_Hash t_Simd128Hash v_K =
     f_shake128_squeeze_three_blocks_pre = (fun (self: t_Simd128Hash) -> true);
     f_shake128_squeeze_three_blocks_post
     =
-    (fun (self: t_Simd128Hash) (out1: (t_Simd128Hash & t_Array (t_Array u8 (sz 504)) v_K)) -> true);
+    (fun (self: t_Simd128Hash) (out4: (t_Simd128Hash & t_Array (t_Array u8 (sz 504)) v_K)) -> true);
     f_shake128_squeeze_three_blocks
     =
     (fun (self: t_Simd128Hash) ->
@@ -229,41 +315,197 @@ let impl (v_K: usize) : Libcrux_ml_kem.Hash_functions.t_Hash t_Simd128Hash v_K =
             )
             v_K
         in
-        let _:Prims.unit =
+        let out0:t_Array u8 (sz 504) = Rust_primitives.Hax.repeat 0uy (sz 504) in
+        let out1:t_Array u8 (sz 504) = Rust_primitives.Hax.repeat 0uy (sz 504) in
+        let out2:t_Array u8 (sz 504) = Rust_primitives.Hax.repeat 0uy (sz 504) in
+        let out3:t_Array u8 (sz 504) = Rust_primitives.Hax.repeat 0uy (sz 504) in
+        let out, out0, out1, out2, out3, self:(t_Array (t_Array u8 (sz 504)) v_K &
+          t_Array u8 (sz 504) &
+          t_Array u8 (sz 504) &
+          t_Array u8 (sz 504) &
+          t_Array u8 (sz 504) &
+          t_Simd128Hash) =
           match cast (v_K <: usize) <: u8 with
           | 2uy ->
-            Rust_primitives.Hax.failure ""
-              "{\n        let Tuple2(out0, out1): tuple2<&mut [[int; 504]], &mut [[int; 504]]> = {\n            core::slice::impl__split_at_mut::<[int; 504]>(rust_primitives::unsize(&mut (out)), 1)\n        };\n        {\n            let _: tuple0 = {\n                libcrux_sha3::neon::x2::incremental::shake128_squeeze_first_three_blocks(\n                    &mut (deref(\n                        &mut (core::ops::index::Index::index(\n                            proj_libcrux_ml_kem::hash_functions::neon::f_shake128_state(self),\n                            0,\n                        )),\n                    )),\n                    rust_primitives::unsize(\n                        &mut (deref(&mut (core::ops::index::Index::index(deref(out0), 0)))),\n                    ),\n                    rust_primitives::unsize(\n                        &mut (deref(&mut (core::ops::index::Index::index(deref(out1), 0)))),\n                    ),\n                )\n            };\n            Tuple0\n        }\n    }"
-
+            let tmp0, tmp1, tmp2:(Libcrux_sha3.Neon.X2.Incremental.t_KeccakState2 &
+              t_Array u8 (sz 504) &
+              t_Array u8 (sz 504)) =
+              Libcrux_sha3.Neon.X2.Incremental.shake128_squeeze_first_three_blocks (self
+                    .f_shake128_state.[ sz 0 ]
+                  <:
+                  Libcrux_sha3.Neon.X2.Incremental.t_KeccakState2)
+                out0
+                out1
+            in
+            let self:t_Simd128Hash =
+              {
+                self with
+                f_shake128_state
+                =
+                Rust_primitives.Hax.Monomorphized_update_at.update_at_usize self.f_shake128_state
+                  (sz 0)
+                  tmp0
+              }
+              <:
+              t_Simd128Hash
+            in
+            let out0:t_Array u8 (sz 504) = tmp1 in
+            let out1:t_Array u8 (sz 504) = tmp2 in
+            let _:Prims.unit = () in
+            let out:t_Array (t_Array u8 (sz 504)) v_K =
+              Rust_primitives.Hax.Monomorphized_update_at.update_at_usize out (sz 0) out0
+            in
+            let out:t_Array (t_Array u8 (sz 504)) v_K =
+              Rust_primitives.Hax.Monomorphized_update_at.update_at_usize out (sz 1) out1
+            in
+            out, out0, out1, out2, out3, self
+            <:
+            (t_Array (t_Array u8 (sz 504)) v_K & t_Array u8 (sz 504) & t_Array u8 (sz 504) &
+              t_Array u8 (sz 504) &
+              t_Array u8 (sz 504) &
+              t_Simd128Hash)
           | 3uy ->
-            let extra:t_Array u8 (sz 504) = Rust_primitives.Hax.repeat 0uy (sz 504) in
-            Rust_primitives.Hax.failure ""
-              "{\n        let Tuple2(out0, out12): tuple2<&mut [[int; 504]], &mut [[int; 504]]> = {\n            core::slice::impl__split_at_mut::<[int; 504]>(rust_primitives::unsize(&mut (out)), 1)\n        };\n        {\n            let Tuple2(out1, out2): tuple2<&mut [[int; 504]], &mut [[int; 504]]> =\n                { core::slice::impl__split_at_mut::<[int; 504]>(&mut (deref(out12)), 1) };\n            {\n                let _: tuple0 = {\n                    libcrux_sha3::neon::x2::incremental::shake128_squeeze_first_three_blocks(\n                        &mut (deref(\n                            &mut (core::ops::index::Index::index(\n                                proj_libcrux_ml_kem::hash_functions::neon::f_shake128_state(self),\n                                0,\n                            )),\n                        )),\n                        rust_primitives::unsize(\n                            &mut (deref(&mut (core::ops::index::Index::index(deref(out0), 0)))),\n                        ),\n                        rust_primitives::unsize(\n                            &mut (deref(&mut (core::ops::index::Index::index(deref(out1), 0)))),\n                        ),\n                    )\n                };\n                {\n                    let _: tuple0 = {\n                        libcrux_sha3::neon::x2::incremental::shake128_squeeze_first_three_blocks(\n                            &mut (deref(\n                                &mut (core::ops::index::Index::index(\n                                    proj_libcrux_ml_kem::hash_functions::neon::f_shake128_state(\n                                        self,\n                                    ),\n                                    1,\n                                )),\n                            )),\n                            rust_primitives::unsize(\n                                &mut (deref(&mut (core::ops::index::Index::index(deref(out2), 0)))),\n                            ),\n                            rust_primitives::unsize(&mut (deref(&mut (extra)))),\n                        )\n                    };\n                    Tuple0\n                }\n            }\n        }\n    }"
-
+            let tmp0, tmp1, tmp2:(Libcrux_sha3.Neon.X2.Incremental.t_KeccakState2 &
+              t_Array u8 (sz 504) &
+              t_Array u8 (sz 504)) =
+              Libcrux_sha3.Neon.X2.Incremental.shake128_squeeze_first_three_blocks (self
+                    .f_shake128_state.[ sz 0 ]
+                  <:
+                  Libcrux_sha3.Neon.X2.Incremental.t_KeccakState2)
+                out0
+                out1
+            in
+            let self:t_Simd128Hash =
+              {
+                self with
+                f_shake128_state
+                =
+                Rust_primitives.Hax.Monomorphized_update_at.update_at_usize self.f_shake128_state
+                  (sz 0)
+                  tmp0
+              }
+              <:
+              t_Simd128Hash
+            in
+            let out0:t_Array u8 (sz 504) = tmp1 in
+            let out1:t_Array u8 (sz 504) = tmp2 in
+            let _:Prims.unit = () in
+            let tmp0, tmp1, tmp2:(Libcrux_sha3.Neon.X2.Incremental.t_KeccakState2 &
+              t_Array u8 (sz 504) &
+              t_Array u8 (sz 504)) =
+              Libcrux_sha3.Neon.X2.Incremental.shake128_squeeze_first_three_blocks (self
+                    .f_shake128_state.[ sz 1 ]
+                  <:
+                  Libcrux_sha3.Neon.X2.Incremental.t_KeccakState2)
+                out2
+                out3
+            in
+            let self:t_Simd128Hash =
+              {
+                self with
+                f_shake128_state
+                =
+                Rust_primitives.Hax.Monomorphized_update_at.update_at_usize self.f_shake128_state
+                  (sz 1)
+                  tmp0
+              }
+              <:
+              t_Simd128Hash
+            in
+            let out2:t_Array u8 (sz 504) = tmp1 in
+            let out3:t_Array u8 (sz 504) = tmp2 in
+            let _:Prims.unit = () in
+            let out:t_Array (t_Array u8 (sz 504)) v_K =
+              Rust_primitives.Hax.Monomorphized_update_at.update_at_usize out (sz 0) out0
+            in
+            let out:t_Array (t_Array u8 (sz 504)) v_K =
+              Rust_primitives.Hax.Monomorphized_update_at.update_at_usize out (sz 1) out1
+            in
+            let out:t_Array (t_Array u8 (sz 504)) v_K =
+              Rust_primitives.Hax.Monomorphized_update_at.update_at_usize out (sz 2) out2
+            in
+            out, out0, out1, out2, out3, self
+            <:
+            (t_Array (t_Array u8 (sz 504)) v_K & t_Array u8 (sz 504) & t_Array u8 (sz 504) &
+              t_Array u8 (sz 504) &
+              t_Array u8 (sz 504) &
+              t_Simd128Hash)
           | 4uy ->
-            Rust_primitives.Hax.failure ""
-              "{\n        let Tuple2(out0, out123): tuple2<&mut [[int; 504]], &mut [[int; 504]]> = {\n            core::slice::impl__split_at_mut::<[int; 504]>(rust_primitives::unsize(&mut (out)), 1)\n        };\n        {\n            let Tuple2(out1, out23): tuple2<&mut [[int; 504]], &mut [[int; 504]]> =\n                { core::slice::impl__split_at_mut::<[int; 504]>(&mut (deref(out123)), 1) };\n            {\n                let Tuple2(out2, out3): tuple2<&mut [[int; 504]], &mut [[int; 504]]> =\n                    { core::slice::impl__split_at_mut::<[int; 504]>(&mut (deref(out23)), 1) };\n                {\n                    let _: tuple0 = {\n                        libcrux_sha3::neon::x2::incremental::shake128_squeeze_first_three_blocks(\n                            &mut (deref(\n                                &mut (core::ops::index::Index::index(\n                                    proj_libcrux_ml_kem::hash_functions::neon::f_shake128_state(\n                                        self,\n                                    ),\n                                    0,\n                                )),\n                            )),\n                            rust_primitives::unsize(\n                                &mut (deref(&mut (core::ops::index::Index::index(deref(out0), 0)))),\n                            ),\n                            rust_primitives::unsize(\n                                &mut (deref(&mut (core::ops::index::Index::index(deref(out1), 0)))),\n                            ),\n                        )\n                    };\n                    {\n                        let _: tuple0 = {\n                            libcrux_sha3::neon::x2::incremental::shake128_squeeze_first_three_blocks(\n                                &mut (deref(\n                                    &mut (core::ops::index::Index::index(\n                                        proj_libcrux_ml_kem::hash_functions::neon::f_shake128_state(\n                                            self,\n                                        ),\n                                        1,\n                                    )),\n                                )),\n                                rust_primitives::unsize(\n                                    &mut (deref(\n                                        &mut (core::ops::index::Index::index(deref(out2), 0)),\n                                    )),\n                                ),\n                                rust_primitives::unsize(\n                                    &mut (deref(\n                                        &mut (core::ops::index::Index::index(deref(out3), 0)),\n                                    )),\n                                ),\n                            )\n                        };\n                        Tuple0\n                    }\n                }\n            }\n        }\n    }"
-
+            let tmp0, tmp1, tmp2:(Libcrux_sha3.Neon.X2.Incremental.t_KeccakState2 &
+              t_Array u8 (sz 504) &
+              t_Array u8 (sz 504)) =
+              Libcrux_sha3.Neon.X2.Incremental.shake128_squeeze_first_three_blocks (self
+                    .f_shake128_state.[ sz 0 ]
+                  <:
+                  Libcrux_sha3.Neon.X2.Incremental.t_KeccakState2)
+                out0
+                out1
+            in
+            let self:t_Simd128Hash =
+              {
+                self with
+                f_shake128_state
+                =
+                Rust_primitives.Hax.Monomorphized_update_at.update_at_usize self.f_shake128_state
+                  (sz 0)
+                  tmp0
+              }
+              <:
+              t_Simd128Hash
+            in
+            let out0:t_Array u8 (sz 504) = tmp1 in
+            let out1:t_Array u8 (sz 504) = tmp2 in
+            let _:Prims.unit = () in
+            let tmp0, tmp1, tmp2:(Libcrux_sha3.Neon.X2.Incremental.t_KeccakState2 &
+              t_Array u8 (sz 504) &
+              t_Array u8 (sz 504)) =
+              Libcrux_sha3.Neon.X2.Incremental.shake128_squeeze_first_three_blocks (self
+                    .f_shake128_state.[ sz 1 ]
+                  <:
+                  Libcrux_sha3.Neon.X2.Incremental.t_KeccakState2)
+                out2
+                out3
+            in
+            let self:t_Simd128Hash =
+              {
+                self with
+                f_shake128_state
+                =
+                Rust_primitives.Hax.Monomorphized_update_at.update_at_usize self.f_shake128_state
+                  (sz 1)
+                  tmp0
+              }
+              <:
+              t_Simd128Hash
+            in
+            let out2:t_Array u8 (sz 504) = tmp1 in
+            let out3:t_Array u8 (sz 504) = tmp2 in
+            let _:Prims.unit = () in
+            let out:t_Array (t_Array u8 (sz 504)) v_K =
+              Rust_primitives.Hax.Monomorphized_update_at.update_at_usize out (sz 0) out0
+            in
+            let out:t_Array (t_Array u8 (sz 504)) v_K =
+              Rust_primitives.Hax.Monomorphized_update_at.update_at_usize out (sz 1) out1
+            in
+            let out:t_Array (t_Array u8 (sz 504)) v_K =
+              Rust_primitives.Hax.Monomorphized_update_at.update_at_usize out (sz 2) out2
+            in
+            let out:t_Array (t_Array u8 (sz 504)) v_K =
+              Rust_primitives.Hax.Monomorphized_update_at.update_at_usize out (sz 3) out3
+            in
+            out, out0, out1, out2, out3, self
+            <:
+            (t_Array (t_Array u8 (sz 504)) v_K & t_Array u8 (sz 504) & t_Array u8 (sz 504) &
+              t_Array u8 (sz 504) &
+              t_Array u8 (sz 504) &
+              t_Simd128Hash)
           | _ ->
-            Rust_primitives.Hax.never_to_any (Core.Panicking.panic_fmt (Core.Fmt.impl_2__new_v1 (Rust_primitives.unsize
-                          (let list =
-                              [
-                                "internal error: entered unreachable code: This function can only called be called with N = 2, 3, 4"
-                              ]
-                            in
-                            FStar.Pervasives.assert_norm (Prims.eq2 (List.Tot.length list) 1);
-                            Rust_primitives.Hax.array_of_list 1 list)
-                        <:
-                        t_Slice string)
-                      (Rust_primitives.unsize (Core.Fmt.Rt.impl_1__none ()
-                            <:
-                            t_Array Core.Fmt.Rt.t_Argument (sz 0))
-                        <:
-                        t_Slice Core.Fmt.Rt.t_Argument)
-                    <:
-                    Core.Fmt.t_Arguments)
-                <:
-                Rust_primitives.Hax.t_Never)
+            out, out0, out1, out2, out3, self
+            <:
+            (t_Array (t_Array u8 (sz 504)) v_K & t_Array u8 (sz 504) & t_Array u8 (sz 504) &
+              t_Array u8 (sz 504) &
+              t_Array u8 (sz 504) &
+              t_Simd128Hash)
         in
         let hax_temp_output:t_Array (t_Array u8 (sz 504)) v_K = out in
         self, hax_temp_output <: (t_Simd128Hash & t_Array (t_Array u8 (sz 504)) v_K));
@@ -291,11 +533,17 @@ let impl (v_K: usize) : Libcrux_ml_kem.Hash_functions.t_Hash t_Simd128Hash v_K =
         Rust_primitives.Hax.repeat (Rust_primitives.Hax.repeat 0uy (sz 168) <: t_Array u8 (sz 168))
           v_K
       in
-      let out, self:(t_Array (t_Array u8 (sz 168)) v_K & t_Simd128Hash) =
+      let out0:t_Array u8 (sz 168) = Rust_primitives.Hax.repeat 0uy (sz 168) in
+      let out1:t_Array u8 (sz 168) = Rust_primitives.Hax.repeat 0uy (sz 168) in
+      let out2:t_Array u8 (sz 168) = Rust_primitives.Hax.repeat 0uy (sz 168) in
+      let out3:t_Array u8 (sz 168) = Rust_primitives.Hax.repeat 0uy (sz 168) in
+      let out, out0, out1, out2, out3, self:(t_Array (t_Array u8 (sz 168)) v_K & t_Array u8 (sz 168) &
+        t_Array u8 (sz 168) &
+        t_Array u8 (sz 168) &
+        t_Array u8 (sz 168) &
+        t_Simd128Hash) =
         match cast (v_K <: usize) <: u8 with
         | 2uy ->
-          let out0:t_Array u8 (sz 168) = Rust_primitives.Hax.repeat 0uy (sz 168) in
-          let out1:t_Array u8 (sz 168) = Rust_primitives.Hax.repeat 0uy (sz 168) in
           let tmp0, tmp1, tmp2:(Libcrux_sha3.Neon.X2.Incremental.t_KeccakState2 &
             t_Array u8 (sz 168) &
             t_Array u8 (sz 168)) =
@@ -327,12 +575,13 @@ let impl (v_K: usize) : Libcrux_ml_kem.Hash_functions.t_Hash t_Simd128Hash v_K =
           let out:t_Array (t_Array u8 (sz 168)) v_K =
             Rust_primitives.Hax.Monomorphized_update_at.update_at_usize out (sz 1) out1
           in
-          out, self <: (t_Array (t_Array u8 (sz 168)) v_K & t_Simd128Hash)
+          out, out0, out1, out2, out3, self
+          <:
+          (t_Array (t_Array u8 (sz 168)) v_K & t_Array u8 (sz 168) & t_Array u8 (sz 168) &
+            t_Array u8 (sz 168) &
+            t_Array u8 (sz 168) &
+            t_Simd128Hash)
         | 3uy ->
-          let out0:t_Array u8 (sz 168) = Rust_primitives.Hax.repeat 0uy (sz 168) in
-          let out1:t_Array u8 (sz 168) = Rust_primitives.Hax.repeat 0uy (sz 168) in
-          let out2:t_Array u8 (sz 168) = Rust_primitives.Hax.repeat 0uy (sz 168) in
-          let out3:t_Array u8 (sz 168) = Rust_primitives.Hax.repeat 0uy (sz 168) in
           let tmp0, tmp1, tmp2:(Libcrux_sha3.Neon.X2.Incremental.t_KeccakState2 &
             t_Array u8 (sz 168) &
             t_Array u8 (sz 168)) =
@@ -392,12 +641,13 @@ let impl (v_K: usize) : Libcrux_ml_kem.Hash_functions.t_Hash t_Simd128Hash v_K =
           let out:t_Array (t_Array u8 (sz 168)) v_K =
             Rust_primitives.Hax.Monomorphized_update_at.update_at_usize out (sz 2) out2
           in
-          out, self <: (t_Array (t_Array u8 (sz 168)) v_K & t_Simd128Hash)
+          out, out0, out1, out2, out3, self
+          <:
+          (t_Array (t_Array u8 (sz 168)) v_K & t_Array u8 (sz 168) & t_Array u8 (sz 168) &
+            t_Array u8 (sz 168) &
+            t_Array u8 (sz 168) &
+            t_Simd128Hash)
         | 4uy ->
-          let out0:t_Array u8 (sz 168) = Rust_primitives.Hax.repeat 0uy (sz 168) in
-          let out1:t_Array u8 (sz 168) = Rust_primitives.Hax.repeat 0uy (sz 168) in
-          let out2:t_Array u8 (sz 168) = Rust_primitives.Hax.repeat 0uy (sz 168) in
-          let out3:t_Array u8 (sz 168) = Rust_primitives.Hax.repeat 0uy (sz 168) in
           let tmp0, tmp1, tmp2:(Libcrux_sha3.Neon.X2.Incremental.t_KeccakState2 &
             t_Array u8 (sz 168) &
             t_Array u8 (sz 168)) =
@@ -460,8 +710,19 @@ let impl (v_K: usize) : Libcrux_ml_kem.Hash_functions.t_Hash t_Simd128Hash v_K =
           let out:t_Array (t_Array u8 (sz 168)) v_K =
             Rust_primitives.Hax.Monomorphized_update_at.update_at_usize out (sz 3) out3
           in
-          out, self <: (t_Array (t_Array u8 (sz 168)) v_K & t_Simd128Hash)
-        | _ -> out, self <: (t_Array (t_Array u8 (sz 168)) v_K & t_Simd128Hash)
+          out, out0, out1, out2, out3, self
+          <:
+          (t_Array (t_Array u8 (sz 168)) v_K & t_Array u8 (sz 168) & t_Array u8 (sz 168) &
+            t_Array u8 (sz 168) &
+            t_Array u8 (sz 168) &
+            t_Simd128Hash)
+        | _ ->
+          out, out0, out1, out2, out3, self
+          <:
+          (t_Array (t_Array u8 (sz 168)) v_K & t_Array u8 (sz 168) & t_Array u8 (sz 168) &
+            t_Array u8 (sz 168) &
+            t_Array u8 (sz 168) &
+            t_Simd128Hash)
       in
       let hax_temp_output:t_Array (t_Array u8 (sz 168)) v_K = out in
       self, hax_temp_output <: (t_Simd128Hash & t_Array (t_Array u8 (sz 168)) v_K)
